verification/verus/fail/withdrawal_finalized_identity_quorum.rs
@@ -1,0 +1,10 @@
+use vstd::prelude::*;
+#[path = "../../../canister/bridge-core/src/kernel.rs"] mod kernel;
+
+verus! {
+proof fn one_provider_is_enough()
+    ensures kernel::withdrawal_finalized_identity_quorum_spec(
+        Some((102int, 7int)), None, None) == Some((102int, 7int))
+{}
+}
+fn main() {}
